Wavelet/Seq/Prog.lean
@@ -51,4 +51,105 @@ def Prog.semantics.{u, v, w}
   (i : Fin k) : Semantics.{u, w, max u v w} Op V (sigs i).ι (sigs i).ω
   := Semantics.link (prog i).semantics (Prog.semantics prog ·.toFin)
 
+-- /-- (Strong) induction principal for proving `motive (prog i)` for all `i`. -/
+-- theorem Prog.semantics_induction
+--   [Arity Op] [DecidableEq χ] [InterpConsts V]
+--   {sigs : Sigs k}
+--   {prog : Prog Op χ V sigs}
+--   {motive : (i' : Fin k) → Semantics Op V (sigs i').ι (sigs i').ω → Prop}
+--   (ind : (i : Fin k) →
+--     (∀ (j : Fin i), motive ⟨j, by omega⟩ (prog.semantics _)) →
+--     motive i (prog.semantics i))
+--   (i : Fin k) :
+--     motive i (prog.semantics i)
+--   := sorry
+
+theorem Prog.semantics_state
+  [Arity Op] [DecidableEq χ] [InterpConsts V]
+  {sigs : Sigs k}
+  {prog : Prog Op χ V sigs}
+  {i : Fin k} :
+    (prog.semantics i).S = LinkState (prog i).semantics (Prog.semantics prog ·.toFin)
+  := by
+  rw [Prog.semantics]
+  rfl
+
+@[simp]
+def Prog.unfoldState
+  [Arity Op] [DecidableEq χ] [InterpConsts V]
+  {sigs : Sigs k}
+  {prog : Prog Op χ V sigs}
+  {i : Fin k} :
+    (prog.semantics i).S → LinkState (prog i).semantics (Prog.semantics prog ·.toFin)
+  := cast Prog.semantics_state
+
+@[simp]
+def Prog.foldState
+  [Arity Op] [DecidableEq χ] [InterpConsts V]
+  {sigs : Sigs k}
+  {prog : Prog Op χ V sigs}
+  {i : Fin k} :
+    LinkState (prog i).semantics (Prog.semantics prog ·.toFin) → (prog.semantics i).S
+  := cast Prog.semantics_state.symm
+
+/-- Unfold a `Prog` state to a `LinkState`. -/
+instance
+  [Arity Op] [DecidableEq χ] [InterpConsts V]
+  {sigs : Sigs k}
+  {prog : Prog Op χ V sigs}
+  {i : Fin k} :
+    Coe ((prog.semantics i).S) (LinkState (prog i).semantics (Prog.semantics prog ·.toFin)) where
+  coe := Prog.unfoldState
+
+/-- Fold a `LinkState` into a `Prog` state. -/
+instance
+  [Arity Op] [DecidableEq χ] [InterpConsts V]
+  {sigs : Sigs k}
+  {prog : Prog Op χ V sigs}
+  {i : Fin k} :
+    Coe (LinkState (prog i).semantics (Prog.semantics prog ·.toFin)) ((prog.semantics i).S) where
+  coe := Prog.foldState
+
+@[simp]
+theorem Prog.state_fold_unfold_eq
+  [Arity Op] [DecidableEq χ] [InterpConsts V]
+  {sigs : Sigs k}
+  {prog : Prog Op χ V sigs}
+  {i : Fin k}
+  (s : (prog.semantics i).S) :
+    Prog.foldState (Prog.unfoldState s) = s
+  := by simp
+
+@[simp]
+theorem Prog.state_unfold_fold_eq
+  [Arity Op] [DecidableEq χ] [InterpConsts V]
+  {sigs : Sigs k}
+  {prog : Prog Op χ V sigs}
+  {i : Fin k}
+  (s : LinkState (prog i).semantics (Prog.semantics prog ·.toFin)) :
+    ↑(↑s : (prog.semantics i).S) = s
+  := by simp
+
+theorem Prog.semantics_init_heq
+  [Arity Op] [DecidableEq χ] [InterpConsts V]
+  {sigs : Sigs k}
+  {prog : Prog Op χ V sigs}
+  {i : Fin k} :
+    (prog.semantics i).init ≍
+      LinkState.init (prog i).semantics (Prog.semantics prog ·.toFin)
+  := by
+  rw [Prog.semantics]
+  rfl
+
+theorem Prog.semantics_init
+  [Arity Op] [DecidableEq χ] [InterpConsts V]
+  {sigs : Sigs k}
+  {prog : Prog Op χ V sigs}
+  {i : Fin k} :
+    ↑(prog.semantics i).init =
+      LinkState.init (prog i).semantics (Prog.semantics prog ·.toFin)
+  := by
+  apply cast_eq_iff_heq.mpr
+  exact Prog.semantics_init_heq
+
 end Wavelet.Seq
