Wavelet/Seq/Invariants.lean
@@ -1,0 +1,162 @@
+import Wavelet.Seq.Prog
+
+/-! Some useful invariants of the sequential semantics. -/
+
+namespace Wavelet.Seq
+
+open Semantics
+
+theorem Fn.inv_const_fn
+  [Arity Op]
+  [DecidableEq χ]
+  [InterpConsts V]
+  {fn : Fn Op χ V m n} :
+    fn.semantics.IsInvariant (λ s => s.fn = fn)
+  := by
+  apply Lts.IsInvariantAt.by_induction
+  · simp [Fn.semantics, Config.init]
+  · intros s₁ s₂ l hinv hstep
+    cases hstep <;> simp [hinv]
+
+theorem Prog.step_star_unfold
+  [Arity Op]
+  [DecidableEq χ]
+  [InterpConsts V]
+  {sigs : Sigs k}
+  {prog : Prog Op χ V sigs}
+  {i : Fin k}
+  {tr : Trace (Label Op V (sigs i).ι (sigs i).ω)}
+  {s : (prog.semantics i).S}
+  (hsteps : (prog.semantics i).lts.Star (prog.semantics i).init tr s) :
+    ((prog i).semantics.link (Prog.semantics prog ·.toFin)).lts.Star
+      (LinkState.init (prog i).semantics (Prog.semantics prog ·.toFin))
+      tr (Prog.unfoldState s)
+  := by
+
+  sorry
+
+theorem Prog.is_invariant_unfold
+  [Arity Op]
+  [DecidableEq χ]
+  [InterpConsts V]
+  {sigs : Sigs k}
+  {prog : Prog Op χ V sigs}
+  {i : Fin k}
+  {Inv : (prog.semantics i).S → Prop}
+  (h : ((prog i).semantics.link (Prog.semantics prog ·.toFin)).IsInvariant (Inv ∘ Prog.foldState)) :
+    (prog.semantics i).IsInvariant Inv
+  := by
+  intros s tr hsteps
+  rw [← Prog.state_fold_unfold_eq s] at hsteps ⊢
+  replace hsteps := Prog.step_star_unfold hsteps
+  have := h hsteps
+  simp at this
+  simp [this]
+
+/-- Unfolded version of `Prog.InvConstProg`. -/
+def Prog.InvConstProg'
+  [Arity Op]
+  [DecidableEq χ]
+  [InterpConsts V]
+  {sigs : Sigs k}
+  {prog : Prog Op χ V sigs}
+  {i : Fin k} : ((prog i).semantics.link (Prog.semantics prog ·.toFin)).S → Prop
+  := LinkInv
+    (λ s => s.fn = prog i)
+    (λ op s => Prog.InvConstProg' (Prog.unfoldState s))
+
+def Prog.InvConstProg
+  [Arity Op]
+  [DecidableEq χ]
+  [InterpConsts V]
+  {sigs : Sigs k}
+  {prog : Prog Op χ V sigs}
+  {i : Fin k} : (prog.semantics i).S → Prop
+  := Prog.InvConstProg' ∘ Prog.unfoldState
+
+theorem Prog.inv_const_prog
+  [Arity Op]
+  [DecidableEq χ]
+  [InterpConsts V]
+  {sigs : Sigs k}
+  {prog : Prog Op χ V sigs}
+  (i : Fin k) :
+    (prog.semantics i).IsInvariant Prog.InvConstProg
+  := by
+  apply Prog.is_invariant_unfold
+  exact Lts.IsInvariantAt.imp
+    (by
+      intros s hinv
+      simp [InvConstProg] at hinv ⊢
+      rw [InvConstProg']
+      exact hinv)
+    (link_inv
+      (main := (prog i).semantics)
+      (deps := (Prog.semantics prog ·.toFin))
+      (mainInv := λ s => s.fn = prog i)
+      (depInvs := λ op => Prog.InvConstProg)
+      Fn.inv_const_fn
+      (by
+        intros depOp
+        apply Prog.inv_const_prog))
+  -- apply link_inv
+  -- · sorry
+  -- -- simp [IsInvariant, IsInvariantAt, Lts.IsInvariantAt]
+  -- -- simp [Prog.InvConstProg'.heq]
+  -- -- rw [Prog.semantics]
+  -- sorry
+
+-- theorem Prog.inv_const_prog
+--   [Arity Op]
+--   [DecidableEq χ]
+--   [InterpConsts V]
+--   {sigs : Sigs k}
+--   {prog : Prog Op χ V sigs}
+--   (i : Fin k) :
+--     (Semantics.link (prog i).semantics (Prog.semantics prog ·.toFin)).IsInvariant
+--       (LinkInv (λ s => s.fn = prog i) (λ depOp s => (Prog.castState s).mainState.fn = prog (depOp.toFin)))
+--   := by
+--   -- apply Prog.semantics_induction (motive := λ i sem => sem.IsInvariant Prog.InvConstProg)
+--   -- -- have := Prog.semantics_induction (motive := λ i sem => True)
+--   -- induction i using Prog.semantics_induction with
+--   -- | _ =>
+--   --   sorry
+--   -- apply link_inv
+--   -- · exact Fn.inv_const_fn
+--   -- · intros op
+--   --   apply Prog.inv_const_prog
+--   --   sorry
+
+--   rcases i with ⟨i, hlt⟩
+--   induction i using Nat.strong_induction_on with
+--   | _ i ih =>
+--     apply link_inv
+--     · exact Fn.inv_const_fn
+--     · intros depOp
+--       have : IsInvariantAt _ _ _ := ih depOp.toFin (by simp) (by omega)
+
+--       have : (Semantics.link (prog depOp.toFin).semantics (Prog.semantics prog ·.toFin)).IsInvariant
+--         fun s => s.mainState.fn = prog depOp.toFin
+--         := sorry
+
+--       sorry
+
+--   --   sorry
+--     -- apply Lts.IsInvariantAt.by_induction
+--     -- · simp [Prog.InvConstProg]
+--     --   constructor
+--     --   · rw [Prog.semantics_init, LinkState.init]
+--     --     simp [Fn.semantics, Config.init]
+--     --   · intros depOp
+--     --     rw [Prog.semantics_init, LinkState.init]
+--     --     simp [Fn.semantics, Config.init]
+--     --     have : Semantics.IsInvariant _ _ := ih depOp.toFin (by simp) (by omega)
+--     --     have := this.base.1
+--     --     exact this
+--     -- · intros s₁ s₂ l hinv hstep
+--     --   -- generalize hsem : prog.semantics ⟨i, hlt⟩ = sem
+--     --   -- rw [← hsem] at hstep
+--     --   rw [Prog.semantics]
+--     --   sorry
+
+end Wavelet.Seq
